Weidenbach_Book/IsaSAT_Propagate_Conflict.thy
@@ -497,16 +497,18 @@ lemma set_conflict_wl'_alt_def:
   by (cases S) (auto simp: set_conflict_wl'_def set_conflict_wl_def)
 
 definition set_conflict_wl'_int :: \<open>nat \<Rightarrow> twl_st_wl_heur \<Rightarrow> twl_st_wl_heur nres\<close> where
-  \<open>set_conflict_wl'_int = (\<lambda>C (M, N, U, D, Q, W, vmtf, \<phi>, clvls, cach). do {
+  \<open>set_conflict_wl'_int = (\<lambda>C (M, N, U, D, Q, W, vmtf, \<phi>, clvls, cach, lbd). do {
     let n = zero_uint32_nat;
-    (D, clvls) \<leftarrow> conflict_merge M N C D n;
-    RETURN (M, N, U, D, {#}, W, vmtf, \<phi>, clvls, cach)})\<close>
+    (D, clvls, lbd) \<leftarrow> conflict_merge M N C D n lbd;
+    RETURN (M, N, U, D, {#}, W, vmtf, \<phi>, clvls, cach, lbd)})\<close>
 
 sepref_thm set_conflict_wl'_int_code
   is \<open>uncurry set_conflict_wl'_int\<close>
   :: \<open>[\<lambda>(C, S). get_conflict_wl_heur S = None \<and> C < length (get_clauses_wl_heur S) \<and>
       distinct (get_clauses_wl_heur S ! C) \<and> literals_are_in_\<L>\<^sub>i\<^sub>n (mset (get_clauses_wl_heur S ! C)) \<and>
-      \<not> tautology (mset (get_clauses_wl_heur S ! C))]\<^sub>a
+      \<not> tautology (mset (get_clauses_wl_heur S ! C)) \<and>
+      literals_are_in_\<L>\<^sub>i\<^sub>n_trail (get_trail_wl_heur S) \<and>
+      no_dup (get_trail_wl_heur S)]\<^sub>a
     nat_assn\<^sup>k *\<^sub>a twl_st_heur_assn\<^sup>d \<rightarrow> twl_st_heur_assn\<close>
   supply [[goals_limit=1]]
     lookup_conflict_merge_code_set_conflict[unfolded twl_st_heur_assn_def, sepref_fr_rules]
@@ -522,30 +524,54 @@ prepare_code_thms (in -) set_conflict_wl'_int_code_def
 lemmas set_conflict_wl'_int_code[sepref_fr_rules] =
   set_conflict_wl'_int_code.refine[OF isasat_input_bounded_nempty_axioms]
 
+(* TODO Move *)
+lemma (in -) RES_RETURN_RES3:
+   \<open>SPEC \<Phi> \<bind> (\<lambda>(T, T', T''). RETURN (f T T' T'')) = RES ((\<lambda>(a, b, c). f a b c) ` {T. \<Phi> T})\<close>
+  using RES_RETURN_RES[of \<open>Collect \<Phi>\<close> \<open>\<lambda>(a, b, c). f a b c\<close>]
+  apply (subst (asm)(2) split_prod_bound)
+  apply (subst (asm)(3) split_prod_bound)
+  by auto
+
+lemma (in -) RES_RES3_RETURN_RES:
+   \<open>RES A \<bind> (\<lambda>(T, T', T''). RES (f T T' T'')) = RES (\<Union>((\<lambda>(a, b, c). f a b c) ` A))\<close>
+  by (auto simp:  pw_eq_iff refine_pw_simps uncurry_def)
+(* End Move *)
+
 lemma set_conflict_wl'_int_set_conflict_wl':
   \<open>(uncurry set_conflict_wl'_int, uncurry (RETURN oo set_conflict_wl')) \<in>
     nat_rel \<times>\<^sub>r twl_st_heur \<rightarrow>\<^sub>f \<langle>twl_st_heur\<rangle>nres_rel\<close>
   by (intro nres_relI frefI)
-     (auto simp: twl_st_heur_def set_conflict_wl'_int_def set_conflict_wl'_def
-        conflict_merge_def bind_RES_RETURN2_eq RETURN_def[symmetric]
-        counts_maximum_level_def)
+    (auto simp: twl_st_heur_def set_conflict_wl'_int_def set_conflict_wl'_def
+        conflict_merge_def bind_RES_RETURN2_eq RETURN_def RES_RES2_RETURN_RES
+        counts_maximum_level_def RES_RETURN_RES3 RES_RES_RETURN_RES RES_RES3_RETURN_RES
+      intro!: RES_refine)
 
 lemma set_conflict_wl'_int_code_set_conflict_wl'[sepref_fr_rules]:
   \<open>(uncurry set_conflict_wl'_int_code, uncurry (RETURN oo set_conflict_wl')) \<in>
     [\<lambda>(C, S). get_conflict_wl S = None \<and> C < length (get_clauses_wl S) \<and>
       distinct (get_clauses_wl S ! C) \<and> literals_are_in_\<L>\<^sub>i\<^sub>n (mset (get_clauses_wl S ! C)) \<and>
-      \<not> tautology (mset (get_clauses_wl S ! C))]\<^sub>a nat_assn\<^sup>k *\<^sub>a twl_st_assn\<^sup>d \<rightarrow>
+      \<not> tautology (mset (get_clauses_wl S ! C)) \<and>
+      literals_are_in_\<L>\<^sub>i\<^sub>n_trail (get_trail_wl S)]\<^sub>a nat_assn\<^sup>k *\<^sub>a twl_st_assn\<^sup>d \<rightarrow>
     twl_st_assn\<close>
     (is \<open>_ \<in> [?pre]\<^sub>a ?im \<rightarrow> ?f\<close>)
 proof -
   have H: \<open>(uncurry set_conflict_wl'_int_code, uncurry (RETURN \<circ>\<circ> set_conflict_wl'))
   \<in> [comp_PRE (nat_rel \<times>\<^sub>f twl_st_heur) (\<lambda>_. True)
-       (\<lambda>_ (C, S). get_conflict_wl_heur S = None \<and> C < length (get_clauses_wl_heur S) \<and>
-           distinct (get_clauses_wl_heur S ! C) \<and> literals_are_in_\<L>\<^sub>i\<^sub>n (mset (get_clauses_wl_heur S ! C)) \<and>
-           \<not> tautology (mset (get_clauses_wl_heur S ! C)))
-       (\<lambda>_. True)]\<^sub>a
-     hrp_comp (nat_assn\<^sup>k *\<^sub>a twl_st_heur_assn\<^sup>d) (nat_rel \<times>\<^sub>f twl_st_heur) \<rightarrow>
-     hr_comp twl_st_heur_assn twl_st_heur\<close>
+       (\<lambda>_ (C, S).
+           get_conflict_wl_heur S = None \<and>
+           C < length (get_clauses_wl_heur S) \<and>
+           distinct (get_clauses_wl_heur S ! C) \<and>
+           literals_are_in_\<L>\<^sub>i\<^sub>n
+            (mset (get_clauses_wl_heur S ! C)) \<and>
+           \<not> tautology (mset (get_clauses_wl_heur S ! C)) \<and>
+           literals_are_in_\<L>\<^sub>i\<^sub>n_trail
+            (get_trail_wl_heur S) \<and>
+           no_dup (get_trail_wl_heur S))
+       (\<lambda>_. True)]\<^sub>a hrp_comp
+                       (nat_assn\<^sup>k *\<^sub>a twl_st_heur_assn\<^sup>d)
+                       (nat_rel \<times>\<^sub>f
+                        twl_st_heur) \<rightarrow> hr_comp
+           twl_st_heur_assn twl_st_heur\<close>
     (is \<open>_ \<in> [?pre']\<^sub>a ?im' \<rightarrow> ?f'\<close>)
     using hfref_compI_PRE_aux[OF set_conflict_wl'_int_code set_conflict_wl'_int_set_conflict_wl']
     .
@@ -951,6 +977,16 @@ setup \<open>map_theory_claset (fn ctxt => ctxt delSWrapper "split_all_tac")\<cl
 context isasat_input_bounded_nempty
 begin
 
+context
+begin
+
+lemma unit_propagation_inner_loop_body_wl_D_helper:
+  \<open>unit_prop_body_wl_D_inv b ba a \<Longrightarrow> literals_are_in_\<L>\<^sub>i\<^sub>n_trail (get_trail_wl b)\<close>
+  unfolding unit_prop_body_wl_D_inv_def unit_prop_body_wl_inv_def
+  by (rule literals_are_\<L>\<^sub>i\<^sub>n_trail_literals_are_in_\<L>\<^sub>i\<^sub>n[of _ \<open>Some (a, ba)\<close>])
+    auto
+ 
+
 sepref_thm unit_propagation_inner_loop_body_wl_D
   is \<open>uncurry2 ((PR_CONST unit_propagation_inner_loop_body_wl_D) :: nat literal \<Rightarrow> nat \<Rightarrow>
            nat twl_st_wl \<Rightarrow> (nat \<times> nat twl_st_wl) nres)\<close>
@@ -960,6 +996,7 @@ sepref_thm unit_propagation_inner_loop_body_wl_D
     watched_by_app_def[symmetric,simp]
     access_lit_in_clauses_def[simp] unit_prop_body_wl_D_invD'[intro]
     length_rll_def[simp] find_unwatched_not_tauto[dest]
+    unit_propagation_inner_loop_body_wl_D_helper[intro]
   supply undefined_lit_polarity_st_iff[iff]
   unfolding unit_propagation_inner_loop_body_wl_D_def length_rll_def[symmetric] PR_CONST_def
   unfolding watched_by_app_def[symmetric] access_lit_in_clauses_def[symmetric]
@@ -971,6 +1008,8 @@ sepref_thm unit_propagation_inner_loop_body_wl_D
   set_conflict_wl'_alt_def[symmetric] fast_minus_def[symmetric]
   supply [[goals_limit=1]]
   by sepref
+
+end
 
 concrete_definition (in -) unit_propagation_inner_loop_body_wl_D_code
    uses isasat_input_bounded_nempty.unit_propagation_inner_loop_body_wl_D.refine_raw
@@ -1215,7 +1254,8 @@ lemma literals_to_update_wl_empty_heur_literals_to_update_wl_empty:
 lemma literals_to_update_wl_empty_heur_code_literals_to_update_wl_empty[sepref_fr_rules]:
   \<open>(literals_to_update_wl_empty_heur_code, RETURN \<circ> literals_to_update_wl_empty)
      \<in> twl_st_assn\<^sup>k \<rightarrow>\<^sub>a bool_assn\<close>
-  using literals_to_update_wl_empty_heur_code_refine[FCOMP literals_to_update_wl_empty_heur_literals_to_update_wl_empty]
+  using literals_to_update_wl_empty_heur_code_refine[FCOMP
+      literals_to_update_wl_empty_heur_literals_to_update_wl_empty]
   unfolding twl_st_assn_W_list[symmetric]
   .
 
